Adding some ideas

BTree.thy
@@ -1,27 +1,32 @@
 theory BTree                 
-  imports Main "HOL-Data_Structures.Cmp" "HOL-Data_Structures.Tree234_Set"
+  imports Main "HOL-Data_Structures.Cmp" "HOL-Data_Structures.Tree23_Set" "HOL-Data_Structures.Tree234_Set"
 begin
 
 text "General structure:  nat values in the leafs and nat/tree node internal node list (nat always larger than every element in the corresponding subtree)"
 (* definition heavily based on Tree234_Set, Pair structure from ...*)
 (* TODO should all basic definitions be more abstract and use later refinements for implementations *)
+(* TODO to keep the list as pairs, the type for the btrees should be changed to linorder with TOP *)
 
-datatype btree = Leaf | Node "(btree * nat) list"
+
+(* TODO more abstract idea: inside each Btree node is some abstract implementation of a sorted list (i.e. a BST),
+   providing access to a function that returns the element with closest smaller key than a given key*)
+
+datatype 'a btree = Leaf | Node "('a btree * 'a) list"
 
 definition "btree_of_pair = fst"
 definition "sep_of_pair = snd"
 
-fun inorder :: "btree \<Rightarrow> nat list" where
+fun inorder :: "'a btree \<Rightarrow> 'a list" where
 "inorder Leaf = []" |
 "inorder (Node kvs) = (foldr (@) (map (\<lambda> (sub, sep). inorder sub @ [sep]) kvs) [])" 
 
 class height =
 fixes height :: "'a \<Rightarrow> nat"
 
-instantiation btree :: height
+instantiation btree :: (type) height
 begin
 
-fun height_btree :: "btree \<Rightarrow> nat" where
+fun height_btree :: "'a btree \<Rightarrow> nat" where
 "height Leaf = 0" |
 "height (Node kvs) = Suc (fold max (map (height \<circ> fst) kvs) 0)"
 
@@ -33,65 +38,19 @@ end
 lemma set_eq_fold:"Suc (fold max xs 0) = Suc (Max (set (0#xs)))"
   by (metis Max.set_eq_fold)
 
-value "(Node [(Leaf, 1), (Node [(Leaf, 1), (Leaf, 10)], 10), (Leaf, 30), (Leaf, 100)])"
-value "inorder (Node [(Leaf, 1), (Node [(Leaf, 1), (Leaf, 10)], 10), (Leaf, 30), (Leaf, 100)])"
+value "(Node [(Leaf, (1::nat)), (Node [(Leaf, 1), (Leaf, 10)], 10), (Leaf, 30), (Leaf, 100)])"
+value "inorder (Node [(Leaf, (1::nat)), (Node [(Leaf, 1), (Leaf, 10)], 10), (Leaf, 30), (Leaf, 100)])"
 
 fun subtrees where "subtrees xs = (map fst xs)"
 fun seperators where "seperators xs = (map fst xs)"
 
-definition btree_set:: "btree \<Rightarrow> nat set" where 
+definition btree_set:: "'a btree \<Rightarrow> 'a set" where 
   "btree_set = set \<circ> inorder"
 
-fun btree_set_alt:: "btree \<Rightarrow> nat set" where
+fun btree_set_alt:: "'a btree \<Rightarrow> 'a set" where
 "btree_set_alt Leaf = {}" |
 "btree_set_alt (Node t) = set (map snd t) \<union> \<Union> (set (map (btree_set_alt) (subtrees t)))"
 
-
-fun bal:: "btree \<Rightarrow> bool" where
-"bal Leaf = True" |
-"bal (Node t) = ((\<forall>sub \<in> set (subtrees t). bal sub) \<and> (\<exists>h.\<forall>sub \<in> set (subtrees t). h = height sub))"
-
-
-fun btree_list:: "(btree * nat) list \<Rightarrow> bool" where
- "btree_list [] = True" |
- "btree_list ((sub, sep)#xs) = (\<forall>x \<in> btree_set sub. x < sep \<and> btree_list xs )"
-
-
-definition "length_invar k xs = (length xs \<ge> k \<and> length xs \<le> 2*k+1)"
-definition "key_invar xs = (sorted (map snd xs))"
-
-fun k_btree:: "nat \<Rightarrow> btree \<Rightarrow> bool"  where
- "k_btree k Leaf = True"
-| "k_btree k (Node xs) = (length_invar k xs \<and> key_invar xs \<and> btree_list xs \<and> (fold (\<and>) (map (k_btree k \<circ> fst) xs) True))"
-
-fun k_btree_root where
-"k_btree_root k Leaf = True" |
-"k_btree_root k (Node xs) = (key_invar xs \<and> btree_list xs \<and>  (fold (\<and>) (map (k_btree k \<circ> btree_of_pair) xs) True))"
-
-datatype list_result = Nomatch | Subtree btree | Match
-
-fun btree_list_choose where
-"btree_list_choose x [] = Nomatch" |
-"btree_list_choose x ((sub, sep)#xs) = (case cmp x sep of LT \<Rightarrow> Subtree sub | EQ \<Rightarrow> Match | GT \<Rightarrow> btree_list_choose x xs)"
-
-(* the following is what Isabelle requires *)
-lemma [simp]: "btree_list_choose y t = Subtree x2 \<Longrightarrow>
-       size x2 < Suc (size_list (\<lambda>x. Suc (size (fst x))) t)"
-  apply (induction t)
-  apply (auto split: list_result.splits)
-  apply (metis (no_types, lifting) dual_order.strict_trans less_Suc_eq less_add_Suc1 list_result.distinct(5) list_result.inject not_add_less2 not_less_eq)
-  done
-
-
-fun isin where
- "isin y (Leaf) = False" |
- "isin y (Node t) = (case btree_list_choose y t of Nomatch \<Rightarrow> False | Match \<Rightarrow> True | Subtree sub \<Rightarrow> isin y sub)"
-
-
-value "btree_set (Node [(Leaf, 0), (Node [(Leaf, 1), (Leaf, 10)], 12), (Leaf, 30), (Leaf, 100)])"
-value "height (Node [(Leaf, 0), (Node [(Leaf, 1), (Leaf, 10)], 12), (Leaf, 30), (Leaf, 100)])"
-(* a bit weird *)
-value "size (Node [(Leaf, 0), (Node [(Leaf, 1), (Leaf, 10)], 12), (Leaf, 30), (Leaf, 100)])"
 
 
 lemma append_foldr_set: "set (foldr (@) xs []) = \<Union> (set (map set xs))"
@@ -104,43 +63,112 @@ lemma btree_set_set_def: "btree_set t = btree_set_alt t"
    apply(auto simp add: btree_set_def append_foldr_set)
   by (metis image_eqI snd_conv)
 
+fun bal:: "'a btree \<Rightarrow> bool" where
+"bal Leaf = True" |
+"bal (Node t) = ((\<forall>sub \<in> set (subtrees t). bal sub) \<and> (\<exists>h.\<forall>sub \<in> set (subtrees t). h = height sub))"
+
+
+definition ordered:: "('a::linorder) btree \<Rightarrow> bool" where "ordered = sorted \<circ> inorder"
+
+fun k_spread:: "nat \<Rightarrow> 'a btree \<Rightarrow> bool" where
+"k_spread k Leaf = True" |
+"k_spread k (Node t) = ((length t \<ge> k \<and> length t \<le> 2*k+1) \<and> (\<forall>sub \<in> set (subtrees t). k_spread k sub))"
+
+datatype 'a list_result = Nomatch | Subtree "'a btree" | Match
+
+(*TODO: at some point this better be replaced with something binary search like *)
+fun btree_list_choose:: "(('a::linorder) btree\<times>'a) list \<Rightarrow> 'a \<Rightarrow> 'a list_result" where
+"btree_list_choose [] x = Nomatch" |
+"btree_list_choose ((sub, sep)#xs) x = (case cmp x sep of LT \<Rightarrow> Subtree sub | EQ \<Rightarrow> Match | GT \<Rightarrow> btree_list_choose xs x)"
+
+
+(* the following is what Isabelle requires *)
+lemma [simp]: "btree_list_choose t y = Subtree x2 \<Longrightarrow>
+       size x2 < Suc (size_list (\<lambda>x. Suc (size (fst x))) t)"
+  apply (induction t)
+  apply (auto split: list_result.splits)
+  apply (metis (no_types, lifting) dual_order.strict_trans less_Suc_eq less_add_Suc1 list_result.distinct(5) list_result.inject not_add_less2 not_less_eq)
+  done
+
+
+fun isin:: "('a::linorder) btree \<Rightarrow> 'a \<Rightarrow> bool" where
+ "isin (Leaf) y = False" |
+ "isin (Node t) y = (case btree_list_choose t y of Nomatch \<Rightarrow> False | Match \<Rightarrow> True | Subtree sub \<Rightarrow> isin sub y)"
+
+
+value "btree_set (Node [(Leaf, (0::nat)), (Node [(Leaf, 1), (Leaf, 10)], 12), (Leaf, 30), (Leaf, 100)])"
+value "height (Node [(Leaf, (0::nat)), (Node [(Leaf, 1), (Leaf, 10)], 12), (Leaf, 30), (Leaf, 100)])"
+(* a bit weird *)
+value "size (Node [(Leaf, (0::nat)), (Node [(Leaf, 1), (Leaf, 10)], 12), (Leaf, 30), (Leaf, 100)])"
+
+
 lemma child_subset: "p \<in> set t \<Longrightarrow> btree_set (fst p) \<subseteq> btree_set (Node t)"
   apply(induction p arbitrary: t)
    apply(auto simp add: btree_set_def append_foldr_set)
   done
 
 
-lemma some_child_sub: "btree_list_choose y t = Subtree x \<Longrightarrow> x \<in> set (map fst t)"
-  apply(induction y t rule: btree_list_choose.induct)
+lemma some_child_sub: "btree_list_choose t y = Subtree x \<Longrightarrow> x \<in> set (map fst t)"
+  apply(induction t y rule: btree_list_choose.induct)
    apply(simp_all)
   by (metis GT list_result.distinct(5) list_result.inject)
 
-lemma some_child_match: "btree_list_choose y t = Match \<Longrightarrow> y \<in> set (map snd t)"
-  apply(induction y t rule: btree_list_choose.induct)
+lemma some_child_match: "btree_list_choose t y = Match \<Longrightarrow> y \<in> set (map snd t)"
+  apply(induction t y rule: btree_list_choose.induct)
    apply(auto simp add: cmp_def)
   by (metis list_result.distinct(6))
 
-lemma isin_true_not_nomatch: "isin y (Node t) = True \<Longrightarrow> btree_list_choose y t \<noteq> Nomatch"
+lemma isin_true_not_nomatch: "isin (Node t) y = True \<Longrightarrow> btree_list_choose t y \<noteq> Nomatch"
   by auto
 
 
-lemma "isin y n = True \<Longrightarrow> y \<in> btree_set n"
-proof(induction y n rule: isin.induct)
-  case (2 y t)
-  then have "btree_list_choose y t = Match \<or> (\<exists>sub. btree_list_choose y t = Subtree sub)"
+lemma "isin n y = True \<Longrightarrow> y \<in> btree_set n"
+proof(induction n y rule: isin.induct)
+  case (2 t y) 
+  then have "btree_list_choose t y = Match \<or> (\<exists>sub. btree_list_choose t y = Subtree sub)"
     using isin_true_not_nomatch list_result.exhaust by blast
   then show ?case
   proof
-    assume "btree_list_choose y t = Match"
-    then show "y \<in> btree_set (Node t)" using some_child_match btree_set_set_def by auto
+    assume "btree_list_choose t y = Match"
+    then show "y \<in> btree_set (Node t)" using some_child_match btree_set_set_def
+      by (metis UnCI btree_set_alt.simps(2))
   next
-    assume "\<exists>sub. btree_list_choose y t = Subtree sub"
-    then obtain sub where "btree_list_choose y t = Subtree sub" by blast
-    then show "y \<in> btree_set (Node t)"   
-      using some_child_sub btree_set_set_def 2 by force
+    assume "\<exists>sub. btree_list_choose t y = Subtree sub"
+    then obtain sub where sub_tree: "btree_list_choose t y = Subtree sub" by blast
+    then have "sub \<in> set (map fst t)" using some_child_sub by auto
+    also have "y \<in> btree_set sub" using 2 sub_tree by auto
+    ultimately show "y \<in> btree_set (Node t)" 
+      using child_subset by fastforce
   qed
 qed simp
 
+fun sorted_list:: "('a::{linorder, bot}) \<Rightarrow> ('a btree \<times> 'a) list \<Rightarrow> bool" where
+"sorted_list left [] = True" |
+"sorted_list left ((sub, sep)#xs) = ((\<forall>x \<in> btree_set sub. x > left \<and> x < sep) \<and> left < sep \<and> sorted_list sep xs)"
 
+fun sorted_alt:: "('a::{linorder, bot} btree) \<Rightarrow> bool" where
+"sorted_alt Leaf = True" |
+"sorted_alt (Node xs) = (sorted_list bot xs \<and> (\<forall>sub \<in> set (map fst xs). sorted_alt sub))"
+
+lemma sorted_list_part: "sorted_list a xs \<Longrightarrow> sorted (map snd ((t, a)#xs))"
+  apply(induction a xs rule: sorted_list.induct)
+   apply(auto)
+  done
+  
+
+lemma sorted_list_bot: "sorted_list bot xs \<Longrightarrow> sorted (map snd xs)"
+  using sorted_list_part by (cases xs) auto
+
+
+lemma "sorted (inorder t) = sorted_alt t"
+  apply(induction t)
+   apply(auto) 
+sorry
+
+lemma isin_set: "sorted(inorder t) \<Longrightarrow> isin t x = (x \<in> btree_set t)"
+  unfolding btree_set_def 
+  apply (induction t) 
+   apply(auto split: list_result.splits) 
+  sorry
 
 end
